examples/dpe/EngineCore.c
@@ -9,7 +9,7 @@
 bool compare(size_t len, const _array uint8_t *a1, const _array uint8_t *a2)
     _requires(a1._length == len)
     _requires(a2._length == len)
-    _ensures((_slprop) _inline_pulse(pure ($(return) <==> Seq.equal (value_of $(a1)) (value_of $(a2)))))
+    _ensures((_slprop) _inline_pulse(pure ($(return) <==> Seq.equal (array_value_of $(a1)) (array_value_of $(a2)))))
 {
     _ghost_stmt(admit());
     return false;
@@ -20,13 +20,10 @@ bool authenticate_l0_image(const engine_record_t *record)
     bool valid_header_sig = ed25519_verify(record->l0_image_auth_pubkey, record->l0_image_header, record->l0_image_header_size, record->l0_image_header_sig);
     if (valid_header_sig)
     {   
-        // uint8_t scratch[DICE_DIGEST_LEN];
-        uint8_t *scratch = (uint8_t *) calloc(DICE_DIGEST_LEN, sizeof(uint8_t));
+        uint8_t scratch[DICE_DIGEST_LEN];
         //allocate a scratch of size DICE_HASH_ALG here and use it
         hacl_hash(DICE_HASH_ALG, record->l0_binary_size, record->l0_binary, scratch);
-        bool res = compare(DICE_DIGEST_LEN, scratch, record->l0_binary_hash);
-        free(scratch);
-        return res;
+        return compare(DICE_DIGEST_LEN, scratch, record->l0_binary_hash);
     }
     else
     {
@@ -34,16 +31,12 @@ bool authenticate_l0_image(const engine_record_t *record)
     }
 }
 
-void compute_cdi(dice_digest cdi, const uds_array uds, const engine_record_t *record) {
-    // uint8_t uds_digest[DICE_DIGEST_LEN];
-    // uint8_t l0_digest[DICE_DIGEST_LEN];
-    uint8_t *uds_digest = (uint8_t *) calloc(DICE_DIGEST_LEN, sizeof(uint8_t));
-    uint8_t *l0_digest = (uint8_t *) calloc(DICE_DIGEST_LEN, sizeof(uint8_t));
+void compute_cdi(_out dice_digest cdi, const uds_array uds, const engine_record_t *record) {
+    uint8_t uds_digest[DICE_DIGEST_LEN];
+    uint8_t l0_digest[DICE_DIGEST_LEN];
     hacl_hash(DICE_HASH_ALG, UDS_LEN, uds, uds_digest);
     hacl_hash(DICE_HASH_ALG, record->l0_binary_size, record->l0_binary, l0_digest);
     hacl_hmac(DICE_HASH_ALG, cdi, uds_digest, DICE_DIGEST_LEN, l0_digest, DICE_DIGEST_LEN);
-    free(uds_digest);
-    free(l0_digest);
 }
 
 bool engine_main(dice_digest cdi, const uds_array uds, const engine_record_t *record) {
