examples/dpe/HACL.h
@@ -13,11 +13,11 @@ typedef uint8_t *ed25519_sig
 bool ed25519_verify(const ed25519_key pubk, const _array uint8_t *hdr, size_t hdr_len, const ed25519_sig sig)
     _requires(hdr._length == hdr_len);
 
-void hacl_hash(uint8_t alg, size_t src_len, const _array uint8_t *src, dice_digest dst)
+void hacl_hash(uint8_t alg, size_t src_len, const _array uint8_t *src, _out dice_digest dst)
     _requires(src._length == src_len);
 
 
-void hacl_hmac(uint8_t alg, dice_digest dst,
+void hacl_hmac(uint8_t alg, _out dice_digest dst,
     const _array uint8_t *key, size_t key_len,
     const _array uint8_t *msg, size_t msg_len)
     _requires(key._length == key_len)
